proof/invariant-abstract/KHeap_AI.thy
@@ -1631,7 +1631,7 @@ lemma update_sched_context_cte_wp_at [wp]:
   by (wpsimp simp: update_sched_context_def set_object_def cte_wp_at_cases get_object_def)
 
 lemma update_sched_context_refs_of [wp]:
- "\<lbrace>\<lambda>s. P ((state_refs_of s) (p := refs_of (SchedContext val n)))\<rbrace>
+ "\<lbrace>\<lambda>s. P ((state_refs_of s) (p := refs_of_sc val))\<rbrace>
     update_sched_context p val
   \<lbrace>\<lambda>rv s. P (state_refs_of s)\<rbrace>"
   apply (wpsimp simp: update_sched_context_def set_object_def get_object_def)
@@ -1679,17 +1679,9 @@ lemma update_sched_context_respect_device_region [wp]:
 
 lemma update_sched_context_iflive:
   "\<lbrace>\<lambda>s. if_live_then_nonz_cap s \<and>
-        (live (SchedContext val n) \<longrightarrow> ex_nonz_cap_to ptr s)\<rbrace>
+        (live_sc val \<longrightarrow> ex_nonz_cap_to ptr s)\<rbrace>
      update_sched_context ptr val \<lbrace>\<lambda>rv. if_live_then_nonz_cap\<rbrace>"
-  by (wpsimp simp: update_sched_context_def get_object_def live_def obj_at_def is_sc_obj_def
-                   valid_sched_context_size_objsI)
-
-lemma update_sched_context_iflive':
-  "\<lbrace>\<lambda>s. if_live_then_nonz_cap s \<and>
-        ((bound (sc_tcb sc) \<or> bound (sc_yield_from sc) \<or> bound (sc_ntfn sc)
-                                \<or> (sc_replies sc \<noteq> [])) \<longrightarrow> ex_nonz_cap_to ptr s)\<rbrace>
-     update_sched_context ptr sc \<lbrace>\<lambda>rv. if_live_then_nonz_cap\<rbrace>"
-  by (wpsimp simp: update_sched_context_def get_object_def live_def obj_at_def is_sc_obj_def)
+  by (wpsimp simp: update_sched_context_def get_object_def live_def live_sc_def obj_at_def)
 
 lemma update_sched_context_ifunsafe [wp]:
   "\<lbrace>if_unsafe_then_cap\<rbrace> update_sched_context ptr val \<lbrace>\<lambda>rv. if_unsafe_then_cap\<rbrace>"
